more mazza

Mazza.thy
@@ -1,9 +1,13 @@
 theory Mazza
   imports
    "thys/MRBNF_Recursor"
-   "HOL-Library.Stream"
+   "HOL-Library.Linear_Temporal_Logic_on_Streams"
    "HOL-Library.Prefix_Order"
    "HOL-Library.Countable_Set_Type"
+   "HOL-Library.Extended_Nat"
+   "HOL-Cardinals.Cardinals"
+   "HOL-Library.Disjoint_Sets"
+   "HOL-Library.BNF_Corec"
 begin
 
 (*untyped lambda calculus*)
@@ -42,20 +46,7 @@ print_mrbnfs
 
 abbreviation "fv \<equiv> FFVars_lam"
 
-coinductive sdistinct where
-  "x \<notin> sset s \<Longrightarrow> sdistinct s \<Longrightarrow> sdistinct (x ## s)"
-
-lemma sdistinct_stl: "sdistinct s \<Longrightarrow> sdistinct (stl s)"
-  by (erule sdistinct.cases) simp
-
-lemma sdistinct_fromN[simp]: "sdistinct (fromN n)"
-  by (coinduction arbitrary: n) (subst siterate.code,  auto)
-
-lemma sdistinct_smap: "inj_on f (sset s) \<Longrightarrow> sdistinct s \<Longrightarrow> sdistinct (smap f s)"
-  by (coinduction arbitrary: s)
-    (auto simp: smap_ctr stream.set_map inj_on_def stream.set_sel sdistinct_stl elim: sdistinct.cases)
-
-class infinite_regular = 
+class infinite_regular =
   assumes large: "|Field (card_suc natLeq)| \<le>o |UNIV::'a set|" and regular: "regularCard |UNIV::'a set|"
 
 lemma infinite_natLeq: "natLeq \<le>o |A| \<Longrightarrow> infinite A"
@@ -69,60 +60,507 @@ lemma infinite: "infinite (UNIV :: 'a ::infinite_regular set)"
 lemma infinite_ex_inj: "\<exists>f :: nat \<Rightarrow> 'a :: infinite_regular. inj f"
   by (rule infinite_countable_subset[OF infinite, simplified])
 
-typedef 'a dstream = "{xs :: 'a :: infinite_regular stream. sdistinct xs}"
-  by (auto intro!: exI[of _ "smap (SOME f :: nat \<Rightarrow> 'a. inj f) nats"] sdistinct_smap
-    someI_ex[OF infinite_ex_inj])
+(*countably infinite set*)
+typedef 'a :: infinite_regular cinfset = "{X :: 'a set. infinite X \<and> countable X}"
+  morphisms set_cinfset Abs_cinfset
+  using infinite_countable_subset'[OF infinite] by auto
 
-setup_lifting type_definition_dstream
+abbreviation in_cinfset  ("(_/ \<in>\<in> _)" [51, 51] 50) where
+  "x \<in>\<in> X \<equiv> x \<in> set_cinfset X"
 
-lift_definition dsmap :: "('a \<Rightarrow> 'a) \<Rightarrow> 'a dstream \<Rightarrow> 'a :: infinite_regular dstream" is
-  "\<lambda>f xs. if bij f then smap f xs else xs"
-  by (auto simp: bij_def intro!: sdistinct_smap elim: inj_on_subset)
+setup_lifting type_definition_cinfset
 
-lift_definition dsset :: "'a :: infinite_regular dstream \<Rightarrow> 'a set" is "sset" .
+lift_definition image_cinfset :: "('a :: infinite_regular \<Rightarrow> 'a) \<Rightarrow> 'a cinfset \<Rightarrow> 'a cinfset" is
+  "\<lambda>f X. if inj_on f X then f ` X else X"
+  by (auto simp: finite_image_iff)
 
-lift_definition dsnth :: "'a :: infinite_regular dstream \<Rightarrow> nat \<Rightarrow> 'a" (infixl \<open>!#!\<close> 100) is "snth" .
-
-lemma countable_sset:
-  fixes s
-  notes * = LeastI[where P="\<lambda>i. s !! i = s !! _", OF refl]
-  shows "countable (sset s)"
-  unfolding sset_range
-  by (intro countableI[where f="\<lambda>x. LEAST i. snth s i = x"] inj_onI, elim imageE, hypsubst_thin)
-    (rule box_equals[OF _ * *], simp)
-
-mrbnf "'a ::infinite_regular dstream"
-  map: dsmap
-  sets: bound: dsset
+mrbnf "'a ::infinite_regular cinfset"
+  map: image_cinfset
+  sets: bound: set_cinfset
   bd: "card_suc natLeq"
   var_class: infinite_regular
-  subgoal by (rule ext, transfer) (simp add: stream.map_id)
-  subgoal by (rule ext, transfer) (simp add: stream.map_comp)
-  subgoal by transfer (simp cong: stream.map_cong)
-  subgoal by (rule ext, transfer) (simp add: stream.set_map)
+  subgoal by (rule ext, transfer) simp
+  subgoal by (rule ext, transfer) (simp add: image_comp bij_is_inj inj_on_subset[OF _ subset_UNIV])
+  subgoal by transfer (simp add: image_comp bij_is_inj inj_on_subset[OF _ subset_UNIV])
+  subgoal by (rule ext, transfer) (simp add: image_comp bij_is_inj inj_on_subset[OF _ subset_UNIV])
   subgoal by (rule infinite_regular_card_order_card_suc[OF natLeq_card_order natLeq_Cinfinite])
   subgoal
     apply (rule card_suc_greater_set[OF natLeq_card_order])
     apply transfer
-    apply (simp flip: countable_card_le_natLeq add: countable_sset)
+    apply (simp flip: countable_card_le_natLeq)
     done
   subgoal by blast
-  subgoal by (clarsimp, transfer) (auto simp: stream.map_id)
+  subgoal by (clarsimp, transfer) auto
+  done
+
+lift_definition get_cinfset :: "'a :: infinite_regular cinfset \<Rightarrow> nat \<Rightarrow> 'a" is "from_nat_into" .
+
+lemma bij_betw_get_cinfset: "bij_betw (get_cinfset S) UNIV (set_cinfset S)"
+  by transfer (simp add: bij_betw_from_nat_into)
+
+lemma inj_get_cinfset: "inj (get_cinfset S)"
+  by (metis bij_betw_def bij_betw_get_cinfset)
+
+lemma get_cinfset_in: "get_cinfset S n \<in>\<in> S"
+  by (metis bij_betw_def bij_betw_get_cinfset rangeI)
+
+(*countably infinite multiset*)
+typedef 'a cinfmset = "{f :: 'a \<Rightarrow> enat. countable {x. f x \<noteq> 0} \<and>
+  (infinite {x. f x \<noteq> 0} \<or> (\<exists>x. f x = \<infinity>))}"
+  morphisms count_cinfmset Abs_cinfmset
+  by (rule exI[of _ "\<lambda>x. if x = undefined then \<infinity> else 0"]) auto
+
+setup_lifting type_definition_cinfmset
+
+lemma sum_infinite_enat: "finite X \<Longrightarrow> sum g X = (\<infinity> :: enat) \<longleftrightarrow> (\<exists>x \<in> X. g x = \<infinity>)"
+  by (induct X rule: finite_induct) auto
+
+lemma sum_infinite_enat': "finite X \<Longrightarrow>  (\<infinity> :: enat) = sum g X \<longleftrightarrow> (\<exists>x \<in> X. g x = \<infinity>)"
+  by (metis sum_infinite_enat)
+
+lift_definition set_cinfmset :: "'a cinfmset \<Rightarrow> 'a set" is
+  "\<lambda>g. {x. g x \<noteq> 0}" .
+
+abbreviation in_cinfmset  ("(_/ \<in>#\<in> _)" [51, 51] 50) where
+  "x \<in>#\<in> X \<equiv> x \<in> set_cinfmset X"
+
+function count_stream :: "'a stream \<Rightarrow> 'a \<Rightarrow> enat" where
+  "count_stream s x = (if x \<notin> sset s then 0
+     else if (\<forall>n. x \<in> sset (sdrop n s)) then \<infinity>
+     else (if x = shd s then eSuc else id) (count_stream (stl s) x))"
+  by auto
+termination
+  apply (relation "measure (\<lambda>(s, x). LEAST n. x \<notin> sset (sdrop n s))")
+   apply (simp_all add: sset_range image_iff flip: snth.simps(2))
+  apply safe
+  apply (subst (2) Least_Suc)
+    apply auto
+  done
+declare count_stream.simps[simp del]
+
+lemma count_stream_zero_iff:  "count_stream s x = 0 \<longleftrightarrow> x \<notin> sset s"
+  apply (induct s x rule: count_stream.induct)
+  apply (auto simp: count_stream.simps split: if_splits)
+  by (metis stream.sel(1) stream.sel(2) stream.set_cases)
+
+lemma count_stream_infinity_iff: "count_stream s x = \<infinity> \<longleftrightarrow> alw (ev (HLD {x})) s"
+  apply (induct s x rule: count_stream.induct)
+  apply (subst count_stream.simps)
+  apply (auto simp: shd_sset alw_iff_sdrop ev_holds_sset simp flip: holds_eq1 dest: spec[of _ 0])
+  apply (metis (mono_tags, lifting) eSuc_infinity eSuc_inject ev_iff_sdrop sdrop_simps(1) sdrop_stl snth_sset stl_sset)
+  apply (metis (mono_tags, lifting) ev_iff_sdrop sdrop_simps(1) sdrop_stl snth_sset stl_sset)
+  done
+
+lemma count_stream_infinity_iff': "\<infinity> = count_stream s x  \<longleftrightarrow> alw (ev (HLD {x})) s"
+  by (metis count_stream_infinity_iff)
+
+lemma exists_infinite_count: "finite (sset s) \<Longrightarrow> \<exists>x \<in> sset s. count_stream s x = \<infinity>"
+  by (erule pigeonhole_stream[of "sset s" s, folded count_stream_infinity_iff, rotated])
+    (auto simp: alw_iff_sdrop HLD_def)
+
+lift_definition cinfmset :: "'a stream \<Rightarrow> 'a cinfmset" is count_stream
+  apply safe
+   apply (simp add: sset_range count_stream_zero_iff)
+  apply (auto simp: count_stream_zero_iff dest!: exists_infinite_count)
+  apply (metis enat.distinct(2))
+  done
+
+lemma set_cinfmset_cinfmset[simp]: "set_cinfmset (cinfmset s) = sset s"
+  by transfer (auto simp: count_stream_zero_iff)
+
+definition rel_cinfmset where
+  "rel_cinfmset R X Y \<longleftrightarrow> (\<exists>s s'. cinfmset s = X \<and> cinfmset s' = Y \<and> stream_all2 R s s')"
+
+lemma disjE1': "P \<or> Q \<Longrightarrow> (P \<Longrightarrow> \<not> Q \<Longrightarrow> R) \<Longrightarrow> (Q \<Longrightarrow> R) \<Longrightarrow> R"
+  by auto
+lemma disjE2': "P \<or> Q \<Longrightarrow> (P \<Longrightarrow> R) \<Longrightarrow> (Q \<Longrightarrow> \<not> P \<Longrightarrow> R) \<Longrightarrow> R"
+  by auto
+
+lift_definition image_cinfmset :: "('a \<Rightarrow> 'b) \<Rightarrow> 'a cinfmset \<Rightarrow> 'b cinfmset" is
+  "\<lambda>f g y. let X = f -` {y} \<inter> {x. g x \<noteq> 0} in if infinite X then \<infinity> else sum g X"
+  subgoal for f g
+    apply (erule conj_mono[rule_format, rotated -1])
+     apply (auto simp: Let_def) []
+     apply (drule countable_image[of _ f])
+     apply (erule countable_subset[rotated])
+     apply auto []
+     apply (smt (verit, best) disjoint_iff_not_equal finite.simps image_iff vimage_singleton_eq)
+    apply (erule disjE1')
+     apply (auto simp: Let_def sum_infinite_enat)
+     apply (erule contrapos_np)
+     apply simp
+     apply (rule finite_subset[rotated])
+      apply (rule finite_UN[THEN iffD2])
+       apply assumption
+      apply (rule ballI)
+      apply (erule spec)
+     apply auto
+    apply fastforce
+    done
+  done
+
+lemma count_image_cinfmset:
+  \<open>count_cinfmset (image_cinfmset f A) x =
+   (if infinite (f -` {x} \<inter> set_cinfmset A) then \<infinity>
+   else (\<Sum>y\<in>f -` {x} \<inter> set_cinfmset A. count_cinfmset A y))\<close>
+  by transfer auto
+
+lemma cinfmset_eqI: "(\<forall>x. count_cinfmset A x = count_cinfmset B x) \<Longrightarrow> A = B"
+  by transfer auto
+
+lemma cinfmset_set_map: "set_cinfmset (image_cinfmset f A) = f ` set_cinfmset A"
+  apply transfer
+  apply (auto simp: Let_def image_iff)
+    apply (metis (mono_tags, lifting) disjoint_iff_not_equal finite.emptyI mem_Collect_eq vimage_singleton_eq)
+  apply (metis (mono_tags, lifting) disjoint_iff_not_equal finite.emptyI mem_Collect_eq vimage_singleton_eq)
+  done
+
+lemma cinfmset_map_comp: "image_cinfmset f (image_cinfmset g A) = image_cinfmset (f o g) A"
+  apply (rule cinfmset_eqI)
+  apply (auto simp: count_image_cinfmset sum_infinite_enat sum_infinite_enat' cinfmset_set_map
+      simp flip: vimage_comp)
+    apply (drule finite_imageI[of _ g])
+    apply (erule notE)
+    apply (erule finite_subset[rotated])
+    apply auto []
+   apply (erule contrapos_np)
+   apply auto []
+   apply (rule finite_subset[rotated])
+    apply (rule finite_UN[THEN iffD2])
+     apply assumption
+    apply (rule ballI)
+    apply (drule bspec)
+     apply assumption
+    apply (erule conjunct1)
+   apply auto []
+  apply (subst sum.If_cases)
+   apply assumption
+  apply (auto simp: of_nat_eq_enat sum_infinite_enat sum_infinite_enat')
+  subgoal
+    apply (rule trans[OF _ sum.group[where g=g]])
+       apply (rule sum.cong[OF refl])
+       apply (rule sum.cong[OF _ refl])
+       apply auto []
+      apply assumption
+     apply blast
+    apply blast
+    done
+  apply (smt (verit, del_insts) Int_assoc Int_insert_right_if1 Int_left_commute finite_Int inf_bot_right insertI1 vimageI2 vimage_Int)
+  done
+
+lemma eSuc_infinity_iff: "eSuc x = \<infinity> \<longleftrightarrow> x = \<infinity>"
+  by (cases x) (auto simp: eSuc_enat)
+
+lemma pigeonhole_stream_strong:
+  assumes "alw (ev (HLD s)) \<omega>"
+  assumes "finite s"
+  shows "\<exists>x\<in>s. alw (ev (HLD {x})) \<omega>"
+proof -
+  obtain S where "infinite S" "\<forall>i \<in> S. \<exists>x\<in>s. \<omega> !! i = x"
+    using \<open>alw (ev (HLD s)) \<omega>\<close>
+    apply atomize_elim
+    apply (auto simp add: alw_iff_sdrop ev_iff_sdrop HLD_iff le_iff_add choice_iff)
+    by (metis infinite_nat_iff_unbounded_le le_add1 sdrop_snth vimage_eq)
+  from pigeonhole_infinite_rel[OF this(1) \<open>finite s\<close> this(2)]
+  show ?thesis
+    by (auto simp add: HLD_iff simp flip: infinite_iff_alw_ev)
+qed
+
+lemma exist_infinite_preimage:
+  "finite (f -` {x} \<inter> sset s) \<Longrightarrow> \<forall>n. \<exists>y\<in>sset (sdrop n s). x = f y \<Longrightarrow>
+  \<exists>y. x = f y \<and> alw (ev (HLD {y})) s"
+  using pigeonhole_stream_strong[of "f -` {x} \<inter> sset s" s]
+  apply (auto simp: alw_iff_sdrop ev_iff_sdrop HLD_iff sset_range sdrop_snth)
+  apply (metis IntD1 vimage_singleton_eq)
+  done
+
+lemma count_stream_smap: "finite (f -` {x} \<inter> sset s) \<Longrightarrow>
+  count_stream (smap f s) x = sum (count_stream s) (f -` {x} \<inter> sset s)"
+  apply (induct "smap f s" x arbitrary: s rule: count_stream.induct)
+  apply (subst (1 2) count_stream.simps[abs_def])
+  apply (auto simp: stream.set_map image_iff shd_sset sum_infinite_enat' intro: sum.neutral)
+  subgoal for s x
+    apply (drule (1) exist_infinite_preimage)
+    apply (auto)
+    by (metis (no_types, opaque_lifting) IntI alw_ev_stl count_stream.elims count_stream_infinity_iff eSuc_infinity i0_ne_infinity vimage_singleton_eq)
+  subgoal premises prems for s n x
+    using prems(2-)
+    apply (subst prems(1))
+        apply (auto elim!: finite_subset[rotated] stream.set_sel(2))
+    apply (subst (2) sum.remove[of _ "shd s"])
+      apply (auto simp: shd_sset sum.If_cases)
+     apply metis
+    apply (subst card_0_eq[THEN iffD2])
+      apply (auto elim!: finite_subset[rotated] stream.set_sel(2))
+     apply metis
+    apply (subst (3) Int_absorb2)
+     apply auto
+     apply metis
+    apply (cases "shd s \<in> sset (stl s)")
+     apply (subst sum.remove[of _ "shd s"])
+       apply (auto simp: iadd_Suc elim!: finite_subset[rotated] stream.set_sel(2)
+        intro!: sum.cong)
+     apply (metis stream.sel(1) stream.sel(2) stream.set_cases)
+    apply (subst count_stream_zero_iff[THEN iffD2, of "shd s"])
+     apply assumption
+    apply (auto intro!: sum.cong elim!: stream.set_sel(2))
+    apply (metis stream.sel(1) stream.sel(2) stream.set_cases)
+    done
+  subgoal for s x
+    apply (drule (1) exist_infinite_preimage)
+    apply (auto)
+    by (metis (no_types, opaque_lifting) IntI alw_ev_stl count_stream.elims count_stream_infinity_iff i0_ne_infinity vimage_singleton_eq)
+  subgoal premises prems for s n x
+    using prems(2-)
+    apply (subst prems(1))
+        apply (auto elim!: finite_subset[rotated] stream.set_sel(2))
+      apply (auto simp: shd_sset sum.If_cases)
+    apply (subst card_0_eq[THEN iffD2])
+      apply (auto elim!: finite_subset[rotated] stream.set_sel(2))
+     apply metis
+    apply (subst (3) Int_absorb2)
+     apply auto
+     apply metis
+    apply (rule sum.cong)
+     apply auto
+    apply (auto intro!: sum.cong elim!: stream.set_sel(2))
+    apply (metis stream.sel(1) stream.sel(2) stream.set_cases)
+    done
+  done
+
+lemma image_cinfmset_cinfmset[simp]: "image_cinfmset f (cinfmset s) = cinfmset (smap f s)"
+  by transfer
+    (auto simp: fun_eq_iff Let_def count_stream_infinity_iff' count_stream_zero_iff sset_range
+    infinite_iff_alw_ev[symmetric] count_stream_smap simp flip: holds_eq1 intro: finite_surj[of _ _ "snth _"])
+
+lift_definition NATS_cinfmset :: "nat cinfmset" is "\<lambda>x::nat. 1"
+  by auto
+
+definition "spermute \<pi> s = smap (\<lambda>i. snth s (\<pi> i)) nats"
+
+lemma sset_spermute: "bij \<pi> \<Longrightarrow> sset (spermute \<pi> s) = sset s"
+  apply (auto simp: spermute_def stream.set_map sset_range image_iff)
+  apply (metis bij_pointE)
+  done
+
+lemma count_stream_fromN: "count_stream (fromN n) x = (if x < n then 0 else 1)"
+  apply (induct "fromN n" x arbitrary: n rule: count_stream.induct)
+  apply (subst count_stream.simps)
+  apply (auto simp: count_stream_zero_iff one_eSuc not_less)
+  using add_leD1 linorder_not_le apply blast
+  done
+
+lemma count_stream_alt: "count_stream s x = (let I = (!!) s -` {x} in if infinite I then \<infinity> else card I)"
+  apply (cases "count_stream s x = \<infinity>")
+   apply (auto simp: count_stream_infinity_iff Let_def alw_iff_sdrop ev_iff_sdrop HLD_iff
+      infinite_nat_iff_unbounded_le)
+    apply (metis le_add1)
+   apply (metis le_iff_add)
+  apply (subst stream_smap_nats)
+  apply (subst count_stream_smap)
+   apply (auto simp: Let_def count_stream_fromN of_nat_eq_enat)
+  apply (meson infinite_nat_iff_unbounded_le vimage_singleton_eq)
+  done
+
+lemma count_stream_spermute:
+  "bij \<pi> \<Longrightarrow> count_stream (spermute \<pi> s) x = count_stream s x"
+  unfolding spermute_def
+  apply (cases "count_stream s x = \<infinity>")
+   apply simp
+   apply (auto simp: count_stream_infinity_iff alw_iff_sdrop ev_iff_sdrop HLD_iff) []
+  subgoal for m
+    apply (rule ccontr)
+    apply simp
+    apply (cases m)
+     apply simp
+     apply (metis bij_pointE)
+    apply (subgoal_tac "finite {i. s !! i = x}")
+     apply (metis (mono_tags, lifting) infinite_nat_iff_unbounded_le le_add1 mem_Collect_eq)
+    apply (subgoal_tac "finite {i. s !! \<pi> i = x}")
+     apply (erule finite_surj[of _ _ "\<pi>"])
+     apply (auto simp: image_iff) []
+     apply (metis bij_pointE)
+    apply (rule finite_subset[of _ "{0 ..< m}"])
+     apply auto
+    apply (metis add.commute less_natE not_less_eq)
+    done
+  apply (auto simp: count_stream_infinity_iff alw_iff_sdrop ev_iff_sdrop HLD_iff) []
+  subgoal for m
+    apply (subst count_stream_smap)
+     apply auto
+     apply (rule finite_subset[of _ "{0 ..< Suc (Max (\<pi> -` {0 ..< m}))}"])
+      apply (auto simp: less_Suc_eq_le count_stream_fromN)
+     apply (metis Max.coboundedI atLeastLessThan_iff finite_atLeastLessThan finite_vimage_iff le_iff_add less_eq_nat.simps(1) linorder_not_less vimageI2)
+    subgoal
+      apply (subst count_stream_alt)
+      apply (auto simp: Let_def of_nat_eq_enat)
+       apply (metis infinite_nat_iff_unbounded_le less_eqE vimage_singleton_eq)
+      apply (subgoal_tac "card ((\<lambda>i. s !! \<pi> i) -` {x}) = card ((\<lambda>i. s !! i) -` {x})")
+       prefer 2
+       apply (rule card_bij[of \<pi> _ _ "inv \<pi>"])
+            apply (auto simp: inj_on_def)
+      apply (rule finite_subset[of _ "{0 ..< Suc (Max (\<pi> -` {0 ..< m}))}"])
+       apply (auto simp: less_Suc_eq_le)
+      apply (metis Max.coboundedI atLeastLessThan_iff finite_atLeastLessThan finite_vimage_iff le_iff_add less_eq_nat.simps(1) linorder_not_less vimageI2)
+      done
+    done
+  done
+
+lemma count_stream_flat: "\<exists>!xs \<in> sset s. x \<in> set xs \<Longrightarrow>
+   \<forall>xs \<in> sset s. \<exists>z. \<exists>n > 0. xs = replicate n z \<Longrightarrow>
+   count_stream (flat s) x = length (THE xs. xs \<in> sset s \<and> x \<in> set xs)"
+  apply (subst count_stream_alt)
+  apply (auto simp: Let_def)
+  sorry
+
+lemma ex_cinfmset: "\<exists>xs. cinfmset xs = X"
+  apply transfer
+  subgoal for f
+    apply (elim conjE exE disjE1')
+    apply (frule (1) bij_betw_from_nat_into)
+    subgoal
+       apply (rule exI[of _ "flat (smap (\<lambda>i.
+         let x = from_nat_into {x. f x \<noteq> 0} i in replicate (the_enat (f x)) x) nats)"])
+      apply (rule ext)
+      subgoal for z
+        apply (cases "f z = 0")
+         apply (auto simp: count_stream_zero_iff)
+         apply (subst (asm) sset_flat)
+          apply (auto simp: stream.set_map Let_def zero_enat_def) [2]
+        apply (smt (verit) bij_betw_def mem_Collect_eq neq0_conv rangeI the_enat.simps)
+      apply (subst count_stream_flat)
+          apply (auto simp: stream.set_map Let_def)
+           apply (metis (mono_tags, lifting) enat_0_iff(2) from_nat_into_surj mem_Collect_eq the_enat.simps zero_less_iff_neq_zero)
+         apply (metis (mono_tags, lifting) Collect_empty_eq enat_0_iff(2) from_nat_into mem_Collect_eq the_enat.simps zero_less_iff_neq_zero)
+        apply (rule the1I2)
+          apply (auto simp: stream.set_map Let_def)
+           apply (metis (mono_tags, lifting) enat_0_iff(2) from_nat_into_surj mem_Collect_eq the_enat.simps zero_less_iff_neq_zero)
+        apply (metis (mono_tags, lifting) the_enat.simps)
+        done
+      done
+term smerge
+  done
+
+lemma cinfmset_eq_iff_spermute: "cinfmset xs' = cinfmset xs \<longleftrightarrow> (\<exists>\<pi>. bij \<pi> \<and> spermute \<pi> xs = xs')"
+  apply transfer
+  apply (auto simp: count_stream_spermute fun_eq_iff)
+  apply (auto simp: count_stream_alt Let_def split: if_splits)
+  sledgehammer
+  sorry
+
+lemma szip_smap_same: "szip (smap f s) (smap g s) = smap (\<lambda>x. (f x, g x)) s"
+  by (coinduction arbitrary: s) auto
+
+lemma spermute_szip: "spermute \<pi> (szip xs ys) = szip (spermute \<pi> xs) (spermute \<pi> ys)"
+  by (auto simp: spermute_def szip_smap_same)
+
+lemma ex_cinfmset_zip_left:
+  assumes "cinfmset xs' = cinfmset xs"
+  shows "\<exists>ys'. cinfmset (szip xs' ys') = cinfmset (szip xs ys)"
+  using assms unfolding cinfmset_eq_iff_spermute
+  apply (elim exE conjE)
+  subgoal for \<pi>
+    by (auto simp: spermute_szip intro!: exI[of _ "spermute \<pi> ys"] exI[of _ \<pi>])
+  done
+
+lemma stream_all2_szipI: "(\<forall>(x, y) \<in> sset (szip xs ys). P x y) \<Longrightarrow> stream_all2 P xs ys"
+  apply (coinduction arbitrary: xs ys)
+  apply auto
+  apply (metis shd_sset szip.simps(1))
+  apply (metis stl_sset szip.simps(2))
+  done
+
+lemma stream_all2_szipD: "xy \<in> sset (szip xs ys) \<Longrightarrow> stream_all2 P xs ys \<Longrightarrow> P (fst xy) (snd xy)"
+  apply (induct xy "szip xs ys" arbitrary: xs ys rule: stream.set_induct)
+  subgoal for h t xs ys
+    by (metis fst_conv snd_conv stream.rel_sel stream.sel(1) szip.simps(1))
+  subgoal for h t xy xs ys
+    by (metis stream.rel_sel stream.sel(2) szip.simps(2))
+  done
+
+lemma stream_all2_iff: "stream_all2 P xs ys \<longleftrightarrow> (\<forall>(x, y) \<in> sset (szip xs ys). P x y)"
+  by (metis split_beta stream_all2_szipD stream_all2_szipI)
+
+lemma stream_all2_reorder_left_invariance:
+  assumes rel: "stream_all2 R xs ys" and ms_x: "cinfmset xs' = cinfmset xs"
+  shows "\<exists>ys'. stream_all2 R xs' ys' \<and> cinfmset ys' = cinfmset ys"
+proof -
+  from ms_x obtain ys' where
+    ms_xy: "cinfmset (szip xs' ys') = cinfmset (szip xs ys)"
+    by (metis ex_cinfmset_zip_left)
+  have "stream_all2 R xs' ys'"
+    using assms(1) ms_xy unfolding stream_all2_iff
+    by (auto dest!: arg_cong[of _ _ set_cinfmset])
+  moreover have "cinfmset ys' = cinfmset ys"
+    using ms_xy
+    apply (subst smap_szip_snd[of "\<lambda>x. x" xs' ys', unfolded stream.map_ident, symmetric])
+    apply (subst smap_szip_snd[of "\<lambda>x. x" xs ys, unfolded stream.map_ident, symmetric])
+    apply (auto simp flip: image_cinfmset_cinfmset)
+    done
+  ultimately show ?thesis
+    by blast
+qed
+
+bnf "'a cinfmset"
+  map: image_cinfmset
+  sets: set_cinfmset
+  bd: "card_suc natLeq"
+  rel: rel_cinfmset
+  subgoal by (rule ext, transfer) (auto simp: fun_eq_iff Int_insert_left)
+  subgoal by (simp add: cinfmset_map_comp fun_eq_iff)
+  subgoal
+    apply transfer
+    apply (auto simp: fun_eq_iff Let_def sum_infinite_enat sum_infinite_enat' intro!: sum.cong)
+    apply (metis (mono_tags, lifting) mem_Collect_eq vimage_inter_cong)
+    apply (metis (mono_tags, lifting) mem_Collect_eq vimage_inter_cong)
+    apply (metis (mono_tags, lifting) mem_Collect_eq vimage_inter_cong)
+    apply (metis (mono_tags, lifting) mem_Collect_eq vimage_inter_cong)
+    done
+  subgoal by (simp add: cinfmset_set_map fun_eq_iff)
+  subgoal
+    using cinfset.bd_card_order by blast
+  subgoal
+    using cinfset.bd_cinfinite by blast
+  subgoal
+    using cinfset.bd_regularCard by blast
+  subgoal
+    apply (rule card_suc_greater_set[OF natLeq_card_order])
+    apply transfer
+    apply (simp flip: countable_card_le_natLeq)
+    done
+  subgoal for R S
+    apply (rule predicate2I)
+    apply (unfold rel_cinfmset_def)
+    apply safe
+    apply (drule stream_all2_reorder_left_invariance[rotated])
+     apply assumption
+    apply (auto simp add: stream.rel_compp relcompp_apply)
+    done
+  subgoal for R
+    unfolding rel_cinfmset_def fun_eq_iff  stream.in_rel
+    apply safe
+    subgoal for x y s s' z
+      by (auto intro!: exI[of _ "cinfmset z"])
+    subgoal for x y z
+      apply (rule exE[OF ex_cinfmset[of z]])
+      apply force
+      done
+    done
   done
 
 (*infinitary untyped lambda calculus*)
 (* binder_datatype 'a ilam =
   Bot
 | Var 'a
-| App "'a ilam" "'a ilam stream"
-| Abs xs::'a dstream t::"'a ilam" binds xs in t
+| App "'a ilam" "'a ilam cinfmset"
+| Abs "X::'a cinfset" "t::'a ilam" binds X in t
 *)
 
 ML \<open>
 val ctors = [
   (("iVar", (NONE : mixfix option)), [@{typ 'var}]),
-  (("iApp", NONE), [@{typ 'rec}, @{typ "'rec stream"}]),
-  (("iAbs", NONE), [@{typ "'bvar dstream"}, @{typ 'brec}])
+  (("iApp", NONE), [@{typ 'rec}, @{typ "'rec cinfmset"}]),
+  (("iAbs", NONE), [@{typ "'bvar cinfset"}, @{typ 'brec}])
 ]
 
 val spec = {
@@ -145,75 +583,100 @@ declare [[mrbnf_internals]]
 local_setup \<open> MRBNF_Sugar.create_binder_datatype spec \<close>
 print_mrbnfs
 
-lemma ex_inj_infinite_regular_var_ilam_pre: "\<exists>f :: 'a :: infinite_regular \<Rightarrow> 'b :: var_ilam_pre. inj f"
-  sorry
+lemma ex_inj_infinite_regular_var_ilam_pre:
+  "\<exists>f :: 'a :: countable \<Rightarrow> 'b :: var_ilam_pre. inj f"
+  unfolding card_of_ordLeq[of UNIV UNIV, simplified]
+  apply (rule ordLeq_transitive[OF _ large])
+  apply (rule ordLeq_transitive[OF countable_card_le_natLeq[THEN iffD1]])
+   apply simp
+  apply (rule natLeq_ordLeq_cinfinite)
+  apply (rule ilam_pre.bd_Cinfinite)
+  done
 
-definition embed :: "'a :: {countable, infinite_regular} \<Rightarrow> 'b :: var_ilam_pre"
+definition embed :: "'a :: countable \<Rightarrow> 'b :: var_ilam_pre"
   ("{{_}}" [999] 1000)  where
   "embed = (SOME f. inj f)"
 
 lemma inj_embed: "inj embed"
   unfolding embed_def
-  apply (rule someI_ex[of inj])
-  apply (insert ex_inj[where 'a='a] infinite_ex_inj[where 'a='a]
-    ex_inj_infinite_regular_var_ilam_pre[where 'a='a and 'b='b])
-  apply (elim exE)
-  subgoal for to_nat to_inf_reg to_var_ilam_pre
-    apply (rule exI[of _ "to_var_ilam_pre o to_inf_reg o to_nat"])
-    apply (rule inj_compose | assumption)+
-    done
-  done
+  by (rule someI_ex[OF ex_inj_infinite_regular_var_ilam_pre[where 'a='a]])
 
 abbreviation "ifv \<equiv> FFVars_ilam"
 
+consts lam_ilam :: "'a :: {countable, var_lam_pre} lam \<Rightarrow> nat list \<Rightarrow> 'b :: var_ilam_pre ilam"  ("\<lbrakk>_\<rbrakk>_" [999, 1000] 1000)
+consts ilam_lam :: "'b :: var_ilam_pre ilam \<Rightarrow> 'a :: {countable, var_lam_pre} lam"  ("\<lparr>_\<rparr>" [999] 1000)
+
+lemma iso_partition_into_countable: "|UNIV :: 'a :: var_ilam_pre set| *c natLeq =o |UNIV :: 'a :: var_ilam_pre set|"
+  by (rule cprod_infinite1'[OF _ Cinfinite_Cnotzero[OF natLeq_Cinfinite]])
+    (simp_all add: var_ilam_pre_class.cinfinite var_sum_class.large)
+
+
+definition iso_partition where
+  "iso_partition = (SOME f:: 'a :: var_ilam_pre \<Rightarrow> nat \<Rightarrow> 'a. bij_betw (case_prod f) UNIV UNIV)"
+
+lemma bij_iso_partition: "bij (case_prod iso_partition :: 'a::var_ilam_pre \<times> nat \<Rightarrow> 'a)"
+  unfolding iso_partition_def using iso_partition_into_countable[where 'a='a]
+  unfolding cprod_def Field_card_of Field_natLeq card_of_ordIso[symmetric] UNIV_prod[symmetric]
+  by (elim exE someI[where P = "\<lambda>f. bij (case_prod f)" and x="\<lambda>x y. _ (x, y)", simplified])
+
+definition var_partition where
+  "var_partition = range (\<lambda>v :: 'a :: var_ilam_pre. range (iso_partition v))"
+
+lemma partition_var_partition: "partition_on UNIV var_partition"
+  unfolding partition_on_def disjoint_def var_partition_def
+  using bij_iso_partition unfolding bij_def surj_def inj_on_def
+  by (auto 5 5)
+
+lemma inj_iso_partition: "inj (iso_partition X)"
+  using bij_iso_partition unfolding bij_def inj_on_def
+  by auto
+
+lemma var_partition_cinf: "X \<in> var_partition \<Longrightarrow> countable X \<and> infinite X"
+  unfolding var_partition_def
+  by (auto intro!: range_inj_infinite[OF inj_iso_partition])
+
+lemma ex1_var_partition: "\<exists>!X. X \<in> var_partition \<and> x \<in> X"
+  using partition_var_partition unfolding partition_on_def disjoint_def by auto
+
+lift_definition super :: "'a ::var_ilam_pre \<Rightarrow> 'a cinfset" ("\<lbrace>_\<rbrace>" [999] 1000) is
+  "\<lambda>x. THE X. X \<in> var_partition \<and> x \<in> X"
+  by (rule the1I2[OF ex1_var_partition]) (auto simp: var_partition_cinf)
+
+lemma in_super: "x \<in>\<in> \<lbrace>x\<rbrace>"
+  by transfer (rule the1I2[OF ex1_var_partition, THEN conjunct2])
+
+lemma super_in: "set_cinfset \<lbrace>x\<rbrace> \<in> var_partition"
+  by transfer (rule the1I2[OF ex1_var_partition, THEN conjunct1])
+
+lemma disjoint_super: "\<lbrace>x\<rbrace> \<noteq> \<lbrace>y\<rbrace> \<Longrightarrow> set_cinfset \<lbrace>x\<rbrace> \<inter> set_cinfset \<lbrace>y\<rbrace> = {}"
+  by (metis Int_emptyI ex1_var_partition set_cinfset_inject super_in)
+
 inductive affine where
   "affine (iVar x)"
-| "affine t \<Longrightarrow> affine (iAbs xx t)"
+| "affine t \<Longrightarrow> affine (iAbs \<lbrace>x\<rbrace> t)"
 | "affine t \<Longrightarrow>
-   \<forall>u \<in> sset uu. affine u \<and> ifv t \<inter> ifv u = {} \<Longrightarrow>
-   \<forall>i j. i < j \<longrightarrow> ifv (uu !! i) \<inter> ifv (uu !! j) = {} \<Longrightarrow>
+   \<forall>u. u \<in>#\<in> uu \<longrightarrow> affine u \<and> ifv t \<inter> ifv u = {} \<Longrightarrow>
+   \<forall>u u'. u \<in>#\<in> uu \<longrightarrow> u' \<in>#\<in> uu \<longrightarrow> u \<noteq> u' \<longrightarrow> ifv u \<inter> ifv u' = {} \<Longrightarrow>
    affine (iApp t uu)"
 
-consts lam_ilam :: "'a :: {countable, infinite_regular, var_lam_pre} lam \<Rightarrow> nat list \<Rightarrow> 'b :: var_ilam_pre ilam"  ("\<lbrakk>_\<rbrakk>_" [999, 1000] 1000)
-consts ilam_lam :: "'b :: var_ilam_pre ilam \<Rightarrow> 'a :: {countable, infinite_regular, var_lam_pre} lam"  ("\<lparr>_\<rparr>" [999] 1000)
-
-
-locale \<VV> =
-  fixes super :: "'b ::var_ilam_pre \<Rightarrow> 'b dstream" ("\<lbrace>_\<rbrace>" [999] 1000)
-  assumes in_super: "x \<in> dsset \<lbrace>x\<rbrace>"
-  and disjoint_super: "\<lbrace>x\<rbrace> \<noteq> \<lbrace>y\<rbrace> \<Longrightarrow> dsset \<lbrace>x\<rbrace> \<inter> dsset \<lbrace>y\<rbrace> = {}"
-begin
-
-inductive renaming (infix "\<approx>" 65) where
-  "\<lbrace>x\<rbrace> = \<lbrace>y\<rbrace> \<Longrightarrow> iVar x \<approx> iVar y"
-| "t \<approx> t' \<Longrightarrow> iAbs \<lbrace>x\<rbrace> t \<approx> iAbs \<lbrace>x\<rbrace> t'"
-| "t \<approx> t' \<Longrightarrow> uu !! 0 \<approx> u' !! 0 \<Longrightarrow> (\<forall>i j. uu !! i \<approx> uu !! j) \<Longrightarrow> (\<forall>i j. uu' !! i \<approx> uu' !! j) \<Longrightarrow>
-   iApp t uu \<approx> iApp t' uu'"
-
-definition uniform where "uniform t = (t \<approx> t)"
-
 lemma lam_ilam_simps[simp]:
-  "\<lbrakk>Var x\<rbrakk>a = iVar (\<lbrace>{{x}}\<rbrace> !#! (list_encode a))"
+  "\<lbrakk>Var x\<rbrakk>a = iVar (get_cinfset \<lbrace>{{x}}\<rbrace> (list_encode a))"
   "\<lbrakk>Abs x M\<rbrakk>a = iAbs \<lbrace>{{x}}\<rbrace> (\<lbrakk>M\<rbrakk>a)"
-  "\<lbrakk>App M N\<rbrakk>a = iApp \<lbrakk>M\<rbrakk>(0#a) (smap (\<lambda>i. \<lbrakk>N\<rbrakk>((i + 1) # a)) nats)"
+  "\<lbrakk>App M N\<rbrakk>a = iApp \<lbrakk>M\<rbrakk>(0#a) (image_cinfmset (\<lambda>i. \<lbrakk>N\<rbrakk>((i + 1) # a)) NATS_cinfmset)"
   sorry
 
-lemma ifv_lam_ilam_disjoint: 
+lemma ifv_lam_ilam_disjoint:
   fixes M N :: "'a :: {countable, infinite_regular, var_lam_pre} lam"
   assumes "\<not>a \<le> a'" "\<not>a' \<le> a"
-  shows "ifv (\<lbrakk>M\<rbrakk>a :: 'b ilam) \<inter> ifv (\<lbrakk>N\<rbrakk>a' :: 'b ilam) = {}"
+  shows "ifv (\<lbrakk>M\<rbrakk>a :: 'b :: var_ilam_pre ilam) \<inter> ifv (\<lbrakk>N\<rbrakk>a' :: 'b ilam) = {}"
   sorry
 
 lemma
   fixes M :: "'a :: {countable, infinite_regular, var_lam_pre} lam"
-  shows "affine (\<lbrakk>M\<rbrakk>a :: 'b ilam)"
+  shows "affine (\<lbrakk>M\<rbrakk>a :: 'b :: var_ilam_pre ilam)"
   by (induct M arbitrary: a)
-    (fastforce simp: stream.set_map intro!: affine.intros
+    (auto simp: cinfmset.set_map intro!: affine.intros
       elim: ifv_lam_ilam_disjoint[unfolded disjoint_iff, rule_format, THEN notE, of _ _ _ _ _ False, rotated 2])+
-
-end
-
-find_theorems list_encode
 
 end
 
@@ -365,7 +828,41 @@ lift_definition map_dlist :: "('a \<Rightarrow> 'a) \<Rightarrow> 'a dlist \<Rig
   by (auto simp: distinct_map bij_def elim: inj_on_subset)
 
 lift_definition set_dlist :: "'a dlist \<Rightarrow> 'a set" is "set" .
-  
+
+coinductive sdistinct where
+  "x \<notin> sset s \<Longrightarrow> sdistinct s \<Longrightarrow> sdistinct (x ## s)"
+
+lemma sdistinct_stl: "sdistinct s \<Longrightarrow> sdistinct (stl s)"
+  by (erule sdistinct.cases) simp
+
+lemma sdistinct_fromN[simp]: "sdistinct (fromN n)"
+  by (coinduction arbitrary: n) (subst siterate.code,  auto)
+
+lemma sdistinct_smap: "inj_on f (sset s) \<Longrightarrow> sdistinct s \<Longrightarrow> sdistinct (smap f s)"
+  by (coinduction arbitrary: s)
+    (auto simp: smap_ctr stream.set_map inj_on_def stream.set_sel sdistinct_stl elim: sdistinct.cases)
+
+typedef 'a dstream = "{xs :: 'a :: infinite_regular stream. sdistinct xs}"
+  by (auto intro!: exI[of _ "smap (SOME f :: nat \<Rightarrow> 'a. inj f) nats"] sdistinct_smap
+    someI_ex[OF infinite_ex_inj])
+
+setup_lifting type_definition_dstream
+
+lift_definition dsmap :: "('a \<Rightarrow> 'a) \<Rightarrow> 'a dstream \<Rightarrow> 'a :: infinite_regular dstream" is
+  "\<lambda>f xs. if bij f then smap f xs else xs"
+  by (auto simp: bij_def intro!: sdistinct_smap elim: inj_on_subset)
+
+lift_definition dsset :: "'a :: infinite_regular dstream \<Rightarrow> 'a set" is "sset" .
+
+lift_definition dsnth :: "'a :: infinite_regular dstream \<Rightarrow> nat \<Rightarrow> 'a" (infixl \<open>!#!\<close> 100) is "snth" .
+
+lemma countable_sset:
+  fixes s
+  notes * = LeastI[where P="\<lambda>i. s !! i = s !! _", OF refl]
+  shows "countable (sset s)"
+  unfolding sset_range
+  by (intro countableI[where f="\<lambda>x. LEAST i. snth s i = x"] inj_onI, elim imageE, hypsubst_thin)
+    (rule box_equals[OF _ * *], simp)
 
 (*polyadic untyped lambda calculus*)
 (* binder_datatype 'a polylc =
