thys/Untyped_Lambda_Calculus/LC.thy
@@ -1,7 +1,7 @@
 theory LC
-imports "../MRBNF_Recursor" "HOL-Library.FSet" 
+imports "../MRBNF_Recursor" "HOL-Library.FSet"
  "../Instantiation_Infrastructure/FixedCountableVars"
-begin 
+begin
 
 (****************************)
 (* 1. GENERAL CUSTOMIZATION *)
@@ -63,7 +63,7 @@ print_mrbnfs
 
 
 (* Monomorphising: *)
-instance var :: var_term_pre apply standard 
+instance var :: var_term_pre apply standard
   using Field_natLeq infinite_iff_card_of_nat infinite_var
   by (auto simp add: regularCard_var)
 
@@ -81,7 +81,7 @@ lemmas SSupp_def = tvSSupp_tvsubst_def
 abbreviation "FFVars \<equiv> FFVars_term"
 (* *)
 
-lemma FFVars_tvsubst[simp]: 
+lemma FFVars_tvsubst[simp]:
 "FFVars (tvsubst \<sigma> t) = (\<Union> {FFVars (\<sigma> x) | x . x \<in> FFVars t})"
 sorry (* AtoDJ: This lemma was no longer available... *)
 
@@ -96,7 +96,7 @@ lemma singl_bound: "|{a}| <o |UNIV::var set|"
   by (rule finite_ordLess_infinite2[OF finite_singleton cinfinite_imp_infinite[OF term_pre.UNIV_cinfinite]])
 
 lemma IImsupp_VVr_empty[simp]: "IImsupp VVr = {}"
-  unfolding IImsupp_def 
+  unfolding IImsupp_def
   term.SSupp_VVr_empty UN_empty Un_empty_left
   apply (rule refl)
   done
@@ -112,13 +112,13 @@ lemma VVr_eq_Var[simp]: "VVr = Var"
 
 lemma tvsubst_VVr_func[simp]: "tvsubst VVr t = t"
   apply (rule term.TT_plain_co_induct)
-  subgoal for x 
+  subgoal for x
     apply (rule case_split[of "isVVr (term_ctor x)"])
      apply (unfold isVVr_def)[1]
      apply (erule exE)
     subgoal premises prems for a
-      unfolding prems  
-      apply (rule term.tvsubst_VVr) 
+      unfolding prems
+      apply (rule term.tvsubst_VVr)
       apply (rule term.SSupp_VVr_bound)
         done
       apply (rule trans)
@@ -270,8 +270,8 @@ lemma Abs_avoid: "|A::var set| <o |UNIV::var set| \<Longrightarrow> \<exists>x' 
   apply assumption
   done
 
-lemma Abs_rrename: 
-"bij (\<sigma>::var\<Rightarrow>var) \<Longrightarrow> |supp \<sigma>| <o |UNIV:: var set| \<Longrightarrow>   
+lemma Abs_rrename:
+"bij (\<sigma>::var\<Rightarrow>var) \<Longrightarrow> |supp \<sigma>| <o |UNIV:: var set| \<Longrightarrow>
  (\<And>a'. a' \<in>FFVars_term e - {a::var} \<Longrightarrow> \<sigma> a' = a') \<Longrightarrow> Abs a e = Abs (\<sigma> a) (rrename_term \<sigma> e)"
 by (metis rrename_simps(3) term.rrename_cong_ids term.set(3))
 
@@ -281,8 +281,8 @@ by (metis rrename_simps(3) term.rrename_cong_ids term.set(3))
 lemma SSupp_upd_bound:
   fixes f::"var \<Rightarrow> trm"
   shows "|SSupp (f (a:=t))| <o |UNIV::var set| \<longleftrightarrow> |SSupp f| <o |UNIV::var set|"
-  unfolding SSupp_def  
-  apply (auto simp only: fun_upd_apply singl_bound ordLeq_refl split: if_splits
+  unfolding SSupp_def
+  apply (auto simp only: fun_upd_apply singl_bound ordLeq_refl fset_simps split: if_splits
       elim!: ordLeq_ordLess_trans[OF card_of_mono1 ordLess_ordLeq_trans[OF term_pre.Un_bound], rotated]
       intro: card_of_mono1)
   done
@@ -299,122 +299,122 @@ lemma supp_swap_bound[simp,intro!]: "|supp (id(x::var := xx, xx := x))| <o |UNIV
 by (simp add: cinfinite_imp_infinite supp_swap_bound term.UNIV_cinfinite)
 
 lemma SSupp_IImsupp_bound: "|SSupp \<sigma>| <o |UNIV:: var set| \<Longrightarrow> |IImsupp \<sigma>| <o |UNIV:: var set|"
-unfolding IImsupp_def 
+unfolding IImsupp_def
 by (simp add: var_ID_class.Un_bound term.set_bd_UNIV var_term_pre_class.UN_bound)
 
 (* *)
 
-lemma IImsupp_tvsubst_su: 
-assumes s[simp]: "|SSupp \<sigma>| <o  |UNIV:: var set|" 
+lemma IImsupp_tvsubst_su:
+assumes s[simp]: "|SSupp \<sigma>| <o  |UNIV:: var set|"
 shows "IImsupp (tvsubst (\<sigma>::var\<Rightarrow>trm) o \<tau>) \<subseteq> IImsupp \<sigma> \<union> IImsupp \<tau>"
 unfolding IImsupp_def SSupp_def apply auto
-by (metis s singletonD term.set(1) term.subst(1)) 
+by (metis s singletonD term.set(1) term.subst(1))
 
-lemma IImsupp_tvsubst_su': 
-assumes s[simp]: "|SSupp \<sigma>| <o  |UNIV:: var set|" 
+lemma IImsupp_tvsubst_su':
+assumes s[simp]: "|SSupp \<sigma>| <o  |UNIV:: var set|"
 shows "IImsupp (\<lambda>a. tvsubst (\<sigma>::var\<Rightarrow>trm) (\<tau> a)) \<subseteq> IImsupp \<sigma> \<union> IImsupp \<tau>"
 using IImsupp_tvsubst_su[OF assms] unfolding o_def .
 
-lemma IImsupp_tvsubst_bound: 
-assumes s: "|SSupp \<sigma>| <o |UNIV:: var set|" "|SSupp \<tau>| <o |UNIV:: var set|" 
+lemma IImsupp_tvsubst_bound:
+assumes s: "|SSupp \<sigma>| <o |UNIV:: var set|" "|SSupp \<tau>| <o |UNIV:: var set|"
 shows "|IImsupp (tvsubst (\<sigma>::var\<Rightarrow>trm) o \<tau>)| <o |UNIV:: var set|"
-using IImsupp_tvsubst_su[OF s(1)] s   
+using IImsupp_tvsubst_su[OF s(1)] s
 by (meson Un_bound SSupp_IImsupp_bound card_of_subset_bound)
 
-lemma SSupp_tvsubst_bound: 
-assumes s: "|SSupp \<sigma>| <o |UNIV:: var set|" "|SSupp \<tau>| <o |UNIV:: var set|" 
+lemma SSupp_tvsubst_bound:
+assumes s: "|SSupp \<sigma>| <o |UNIV:: var set|" "|SSupp \<tau>| <o |UNIV:: var set|"
 shows "|SSupp (tvsubst (\<sigma>::var\<Rightarrow>trm) o \<tau>)| <o |UNIV:: var set|"
-using IImsupp_tvsubst_bound[OF assms] 
+using IImsupp_tvsubst_bound[OF assms]
 by (metis IImsupp_def card_of_subset_bound sup_ge1)
 
-lemma SSupp_tvsubst_bound': 
-assumes s: "|SSupp \<sigma>| <o |UNIV:: var set|" "|SSupp \<tau>| <o |UNIV:: var set|" 
+lemma SSupp_tvsubst_bound':
+assumes s: "|SSupp \<sigma>| <o |UNIV:: var set|" "|SSupp \<tau>| <o |UNIV:: var set|"
 shows "|SSupp (\<lambda>a. tvsubst (\<sigma>::var\<Rightarrow>trm) (\<tau> a))| <o |UNIV:: var set|"
 using SSupp_tvsubst_bound[OF assms] unfolding o_def .
 
 (* *)
 
-lemma IImsupp_rrename_su: 
-assumes s[simp]: "bij (\<sigma>::var\<Rightarrow>var)" "|supp \<sigma>| <o  |UNIV:: var set|" 
+lemma IImsupp_rrename_su:
+assumes s[simp]: "bij (\<sigma>::var\<Rightarrow>var)" "|supp \<sigma>| <o  |UNIV:: var set|"
 shows "IImsupp (rrename_term (\<sigma>::var\<Rightarrow>var) o \<tau>) \<subseteq> imsupp \<sigma> \<union> IImsupp \<tau>"
 unfolding IImsupp_def imsupp_def supp_def SSupp_def by force
 
-lemma IImsupp_rrename_su': 
-assumes s[simp]: "bij (\<sigma>::var\<Rightarrow>var)" "|supp \<sigma>| <o  |UNIV:: var set|" 
+lemma IImsupp_rrename_su':
+assumes s[simp]: "bij (\<sigma>::var\<Rightarrow>var)" "|supp \<sigma>| <o  |UNIV:: var set|"
 shows "IImsupp (\<lambda>a. rrename_term (\<sigma>::var\<Rightarrow>var) (\<tau> a)) \<subseteq> imsupp \<sigma> \<union> IImsupp \<tau>"
 using IImsupp_rrename_su[OF assms] unfolding o_def .
 
-lemma IImsupp_rrename_bound: 
-assumes s: "bij (\<sigma>::var\<Rightarrow>var)" "|supp \<sigma>| <o  |UNIV:: var set|" "|SSupp \<tau>| <o |UNIV:: var set|" 
+lemma IImsupp_rrename_bound:
+assumes s: "bij (\<sigma>::var\<Rightarrow>var)" "|supp \<sigma>| <o  |UNIV:: var set|" "|SSupp \<tau>| <o |UNIV:: var set|"
 shows "|IImsupp (rrename_term (\<sigma>::var\<Rightarrow>var) o \<tau>)| <o |UNIV:: var set|"
 using IImsupp_rrename_su[OF s(1,2)] s
 by (metis SSupp_IImsupp_bound finite_Un finite_iff_le_card_var finite_subset imsupp_supp_bound infinite_var)
 
-lemma SSupp_rrename_bound: 
-assumes s: "bij (\<sigma>::var\<Rightarrow>var)" "|supp \<sigma>| <o  |UNIV:: var set|" "|SSupp \<tau>| <o |UNIV:: var set|"  
+lemma SSupp_rrename_bound:
+assumes s: "bij (\<sigma>::var\<Rightarrow>var)" "|supp \<sigma>| <o  |UNIV:: var set|" "|SSupp \<tau>| <o |UNIV:: var set|"
 shows "|SSupp (rrename_term (\<sigma>::var\<Rightarrow>var) o \<tau>)| <o |UNIV:: var set|"
-using IImsupp_rrename_bound[OF assms] 
+using IImsupp_rrename_bound[OF assms]
 by (metis IImsupp_def card_of_subset_bound sup_ge1)
 
-lemma SSupp_rrename_bound': 
-assumes s: "bij (\<sigma>::var\<Rightarrow>var)" "|supp \<sigma>| <o  |UNIV:: var set|" "|SSupp \<tau>| <o |UNIV:: var set|"  
+lemma SSupp_rrename_bound':
+assumes s: "bij (\<sigma>::var\<Rightarrow>var)" "|supp \<sigma>| <o  |UNIV:: var set|" "|SSupp \<tau>| <o |UNIV:: var set|"
 shows "|SSupp (\<lambda>a. rrename_term (\<sigma>::var\<Rightarrow>var) (\<tau> a))| <o |UNIV:: var set|"
 using SSupp_rrename_bound[OF assms] unfolding o_def .
 
 (* *)
-lemma SSupp_update_rrename_bound: 
+lemma SSupp_update_rrename_bound:
 "|SSupp (Var(\<sigma> (x::var) := rrename_term \<sigma> e))| <o |UNIV::var set|"
 using SSupp_upd_Var_bound .
 
-lemma IImsupp_rrename_update_su: 
+lemma IImsupp_rrename_update_su:
 assumes s[simp]: "bij (\<sigma>::var\<Rightarrow>var)" "|supp \<sigma>| <o |UNIV::var set|"
-shows "IImsupp (rrename_term \<sigma> \<circ> Var(x := e)) \<subseteq> 
+shows "IImsupp (rrename_term \<sigma> \<circ> Var(x := e)) \<subseteq>
        imsupp \<sigma> \<union> {x} \<union> FFVars_term e"
-unfolding IImsupp_def SSupp_def imsupp_def supp_def by (auto split: if_splits)  
+unfolding IImsupp_def SSupp_def imsupp_def supp_def by (auto split: if_splits)
 
-lemma IImsupp_rrename_update_bound: 
+lemma IImsupp_rrename_update_bound:
 assumes s[simp]: "bij (\<sigma>::var\<Rightarrow>var)" "|supp \<sigma>| <o |UNIV::var set|"
 shows "|IImsupp (rrename_term \<sigma> \<circ> Var(x := e))| <o |UNIV::var set|"
-using IImsupp_rrename_update_su[OF assms]  
+using IImsupp_rrename_update_su[OF assms]
 by (meson Un_bound card_of_subset_bound imsupp_supp_bound infinite_var s(2) singl_bound term.set_bd_UNIV)
 
-lemma SSupp_rrename_update_bound: 
+lemma SSupp_rrename_update_bound:
 assumes s[simp]: "bij (\<sigma>::var\<Rightarrow>var)" "|supp \<sigma>| <o |UNIV::var set|"
 shows "|SSupp (rrename_term \<sigma> \<circ> Var(x := e))| <o |UNIV::var set|"
-using IImsupp_rrename_update_bound[OF assms] 
+using IImsupp_rrename_update_bound[OF assms]
   by (metis (mono_tags) IImsupp_def finite_Un finite_iff_le_card_var)
 
 (* Action of swapping (a particular renaming) on variables *)
 
-lemma rrename_swap_Var1[simp]: "rrename_term (id(x := xx, xx := x)) (Var (x::var)) = Var xx" 
+lemma rrename_swap_Var1[simp]: "rrename_term (id(x := xx, xx := x)) (Var (x::var)) = Var xx"
 apply(subst rrename_simps(1)) by auto
-lemma rrename_swap_Var2[simp]: "rrename_term (id(x := xx, xx := x)) (Var (xx::var)) = Var x" 
+lemma rrename_swap_Var2[simp]: "rrename_term (id(x := xx, xx := x)) (Var (xx::var)) = Var x"
 apply(subst rrename_simps(1)) by auto
-lemma rrename_swap_Var3[simp]: "z \<notin> {x,xx} \<Longrightarrow> rrename_term (id(x := xx, xx := x)) (Var (z::var)) = Var z" 
+lemma rrename_swap_Var3[simp]: "z \<notin> {x,xx} \<Longrightarrow> rrename_term (id(x := xx, xx := x)) (Var (z::var)) = Var z"
 apply(subst rrename_simps(1)) by auto
-lemma rrename_swap_Var[simp]: "rrename_term (id(x := xx, xx := x)) (Var (z::var)) = 
+lemma rrename_swap_Var[simp]: "rrename_term (id(x := xx, xx := x)) (Var (z::var)) =
  Var (if z = x then xx else if z = xx then x else z)"
 apply(subst rrename_simps(1)) by auto
 
 (* Compositionality properties of renaming and term-for-variable substitution *)
 
-lemma tvsubst_comp: 
+lemma tvsubst_comp:
 assumes s[simp]: "|SSupp \<sigma>| <o |UNIV:: var set|" "|SSupp \<tau>| <o |UNIV:: var set|"
 shows "tvsubst (\<sigma>::var\<Rightarrow>trm) (tvsubst \<tau> e) = tvsubst (tvsubst \<sigma> \<circ> \<tau>) e"
 proof-
   note SSupp_tvsubst_bound'[OF s, simp]
   show ?thesis
   apply(induct e rule: term.fresh_induct[where A = "IImsupp \<sigma> \<union> IImsupp \<tau>"])
-    subgoal using Un_bound[OF s]  
+    subgoal using Un_bound[OF s]
       using var_ID_class.Un_bound SSupp_IImsupp_bound s(1) s(2) by blast
     subgoal by simp
     subgoal by simp
-    subgoal for x t apply(subgoal_tac "x \<notin> IImsupp (\<lambda>a. tvsubst \<sigma> (\<tau> a))") 
+    subgoal for x t apply(subgoal_tac "x \<notin> IImsupp (\<lambda>a. tvsubst \<sigma> (\<tau> a))")
       subgoal by simp
-      subgoal using IImsupp_tvsubst_su'[OF s(1)] by blast . . 
+      subgoal using IImsupp_tvsubst_su'[OF s(1)] by blast . .
 qed
 
-lemma rrename_tvsubst_comp: 
+lemma rrename_tvsubst_comp:
 assumes b[simp]: "bij (\<sigma>::var\<Rightarrow>var)" and s[simp]: "|supp \<sigma>| <o |UNIV:: var set|" "|SSupp \<tau>| <o |UNIV:: var set|"
 shows "rrename_term \<sigma> (tvsubst \<tau> e) = tvsubst (rrename_term \<sigma> \<circ> \<tau>) e"
 proof-
@@ -422,35 +422,35 @@ proof-
   show ?thesis
   apply(induct e rule: term.fresh_induct[where A = "IImsupp \<tau> \<union> imsupp \<sigma>"])
     subgoal using s(1) s(2) Un_bound SSupp_IImsupp_bound imsupp_supp_bound infinite_var by blast
-    subgoal by simp 
     subgoal by simp
-    subgoal for x t apply simp apply(subgoal_tac "x \<notin> IImsupp (\<lambda>a. rrename_term  \<sigma> (\<tau> a))") 
+    subgoal by simp
+    subgoal for x t apply simp apply(subgoal_tac "x \<notin> IImsupp (\<lambda>a. rrename_term  \<sigma> (\<tau> a))")
       subgoal unfolding imsupp_def supp_def by simp
       subgoal using IImsupp_rrename_su' b s(1) by blast . .
 qed
 
 (* Equivariance of unary substitution: *)
 
-lemma tvsubst_rrename_comp[simp]: 
+lemma tvsubst_rrename_comp[simp]:
 assumes s[simp]: "bij (\<sigma>::var\<Rightarrow>var)" "|supp \<sigma>| <o |UNIV::var set|"
 shows "tvsubst (rrename_term \<sigma> \<circ> Var(x := e2)) e1 = tvsubst (Var(\<sigma> x := rrename_term \<sigma> e2)) (rrename_term \<sigma> e1)"
 proof-
   note SSupp_rrename_update_bound[OF assms, unfolded comp_def, simplified, simp]
-  note SSupp_update_rrename_bound[unfolded fun_upd_def, simplified, simp] 
+  note SSupp_update_rrename_bound[unfolded fun_upd_def, simplified, simp]
   show ?thesis
   apply(induct e1 rule: term.fresh_induct[where A = "{x} \<union> FFVars_term e2 \<union> imsupp \<sigma>"])
-    subgoal by (meson Un_bound imsupp_supp_bound infinite_var s(2) singl_bound term.set_bd_UNIV) 
-    subgoal by auto 
+    subgoal by (meson Un_bound imsupp_supp_bound infinite_var s(2) singl_bound term.set_bd_UNIV)
+    subgoal by auto
     subgoal by simp
-    subgoal for y t apply simp apply(subgoal_tac 
-      "y \<notin> IImsupp ((\<lambda>a. rrename_term \<sigma> (if a = x then e2 else Var a))) \<and> 
-      \<sigma> y \<notin> IImsupp (\<lambda>a. if a = \<sigma> x then rrename_term \<sigma> e2 else Var a)") 
+    subgoal for y t apply simp apply(subgoal_tac
+      "y \<notin> IImsupp ((\<lambda>a. rrename_term \<sigma> (if a = x then e2 else Var a))) \<and>
+      \<sigma> y \<notin> IImsupp (\<lambda>a. if a = \<sigma> x then rrename_term \<sigma> e2 else Var a)")
       subgoal unfolding imsupp_def supp_def by simp
       subgoal unfolding IImsupp_def imsupp_def SSupp_def supp_def by auto . .
 qed
 
 (* Unary substitution versus swapping: *)
-lemma tvsubst_Var_rrename_term: 
+lemma tvsubst_Var_rrename_term:
 assumes xx: "xx \<notin> FFVars_term e1 - {x}"
 shows "tvsubst (Var((x::var) := e2)) e1 = tvsubst (Var(xx := e2)) (rrename_term (id(x := xx, xx := x)) e1)"
 proof-
@@ -459,11 +459,11 @@ proof-
     subgoal by (metis insert_is_Un term.set(1) term.set(2) term.set_bd_UNIV)
     subgoal by simp
     subgoal by auto
-    subgoal for y t apply simp apply(subgoal_tac 
-      "y \<notin> IImsupp (Var(x := e2)) \<and> y \<notin> IImsupp (Var(xx := e2))") 
+    subgoal for y t apply simp apply(subgoal_tac
+      "y \<notin> IImsupp (Var(x := e2)) \<and> y \<notin> IImsupp (Var(xx := e2))")
       subgoal unfolding imsupp_def supp_def by auto
       subgoal unfolding IImsupp_def imsupp_def SSupp_def supp_def by auto . .
 qed
- 
+
 
 end
